\begin{cases} \frac{\sqrt{2} \mu}{2} \theta\left(\lambda^{{\prime\prime}}_{1}\right) & \text{for}\: \lVert {r_{{t}} \rVert} \leq \epsilon \wedge \lVert {u_{{t}} \rVert} \leq \epsilon \\\frac{\mu r_{{t2}} \theta\left(\lambda^{{\prime}}_{1}\right)}{\lVert {r_{{t}} \rVert}} & \text{for}\: \lVert {\Delta} \rVert \leq \epsilon \\- \frac{\theta\left(\lambda_{1}\right)}{2} \left(- \frac{\Delta_{2} \mu}{\lVert {\Delta} \rVert} - \frac{\mu u_{{t2}}}{\lVert {u_{{t}} \rVert}}\right) - \frac{\theta\left(\lambda_{2}\right)}{2} \left(\frac{\Delta_{2} \mu}{\lVert {\Delta} \rVert} - \frac{\mu u_{{t2}}}{\lVert {u_{{t}} \rVert}}\right) & \text{for}\: \lVert {\Delta} \rVert > \epsilon \wedge \lVert {u_{{t}} \rVert} > \epsilon \\\frac{\mu}{4 \lVert {r_{{t}} \rVert}} \left(- 2 r_{{t2}} \theta\left(\lambda^{{\prime}}_{1}\right) + 2 r_{{t2}} \theta\left(\lambda^{{\prime}}_{2}\right) + \sqrt{2 r_{{t1}}^{2} + 2 r_{{t2}}^{2}} \theta\left(\lambda^{{\prime}}_{1}\right) + \sqrt{2 r_{{t1}}^{2} + 2 r_{{t2}}^{2}} \theta\left(\lambda^{{\prime}}_{2}\right)\right) & \text{for}\: \lVert {u_{{t}} \rVert} \leq \epsilon \wedge \lVert {\Delta} \rVert > \epsilon \wedge \lVert {r_{{t}} \rVert} > \epsilon \end{cases}