\begin{cases} \frac{\mu^{2} \left(\mu - 1\right) \theta\left(\lambda^{{\prime\prime}}_{1}\right)}{2 \mu^{2} - 2 \mu + 1} & \text{for}\: \lVert {r_{{t}} \rVert} \leq \epsilon \wedge \lVert {u_{{t}} \rVert} \leq \epsilon \\\frac{\mu r_{{t1}} r_{{t2}} \theta\left(\lambda^{{\prime}}_{1}\right)}{\lVert {r_{{t}} \rVert}^{2}} & \text{for}\: \lVert {\Delta} \rVert \leq \epsilon \\\frac{\Delta_{1} \Delta_{2} \mu \max\left(0, \lambda_{1}\right)}{2 \lVert {\Delta} \rVert^{3}} - \frac{\Delta_{1} \Delta_{2} \mu \max\left(0, \lambda_{2}\right)}{2 \lVert {\Delta} \rVert^{3}} - \frac{\Delta_{1} \theta\left(\lambda_{1}\right)}{2 \lVert {\Delta} \rVert} \left(- \frac{\Delta_{2} \mu}{\lVert {\Delta} \rVert} - \frac{\mu u_{{t2}}}{\lVert {u_{{t}} \rVert}}\right) + \frac{\Delta_{1} \theta\left(\lambda_{2}\right)}{2 \lVert {\Delta} \rVert} \left(\frac{\Delta_{2} \mu}{\lVert {\Delta} \rVert} - \frac{\mu u_{{t2}}}{\lVert {u_{{t}} \rVert}}\right) & \text{for}\: \lVert {\Delta} \rVert > \epsilon \wedge \lVert {u_{{t}} \rVert} > \epsilon \\\frac{\mu r_{{t1}}}{4 \lVert {r_{{t}} \rVert}^{3}} \left(2 \lVert {r_{{t}} \rVert} r_{{t2}} \theta\left(\lambda^{{\prime}}_{1}\right) + 2 \lVert {r_{{t}} \rVert} r_{{t2}} \theta\left(\lambda^{{\prime}}_{2}\right) - \sqrt{2} r_{{t1}}^{2} \theta\left(\lambda^{{\prime}}_{1}\right) + \sqrt{2} r_{{t1}}^{2} \theta\left(\lambda^{{\prime}}_{2}\right) - \sqrt{2} r_{{t2}}^{2} \theta\left(\lambda^{{\prime}}_{1}\right) + \sqrt{2} r_{{t2}}^{2} \theta\left(\lambda^{{\prime}}_{2}\right) + 2 r_{{t2}} \max\left(0, \lambda^{{\prime}}_{1}\right) - 2 r_{{t2}} \max\left(0, \lambda^{{\prime}}_{2}\right)\right) & \text{for}\: \lVert {u_{{t}} \rVert} \leq \epsilon \wedge \lVert {\Delta} \rVert > \epsilon \wedge \lVert {r_{{t}} \rVert} > \epsilon \end{cases}