\begin{cases} \frac{\mu \theta\left(\lambda^{{\prime\prime}}_{1}\right)}{\sqrt{2 \mu^{2} - 2 \mu + 1}} + 1 & \text{for}\: \lVert {r_{{t}} \rVert} \leq \epsilon \wedge \lVert {u_{{t}} \rVert} \leq \epsilon \\1 + \frac{r_{{t2}} \theta\left(\lambda^{{\prime}}_{1}\right)}{\lVert {r_{{t}} \rVert}} & \text{for}\: \lVert {\Delta} \rVert \leq \epsilon \wedge \lVert {r_{{t}} \rVert} > \epsilon \wedge \lVert {u_{{t}} \rVert} > \epsilon \\- \frac{\Delta_{2}^{2} \theta\left(\lambda_{1}\right)}{2 \lVert {\Delta} \rVert^{2}} - \frac{\Delta_{2}^{2} \theta\left(\lambda_{2}\right)}{2 \lVert {\Delta} \rVert^{2}} - \frac{\max\left(0, \lambda_{2}\right)}{2} \left(- \frac{\Delta_{2}^{2}}{\lVert {\Delta} \rVert^{3}} + \frac{1}{\lVert {\Delta} \rVert}\right) - \frac{\max\left(0, \lambda_{1}\right)}{2} \left(\frac{\Delta_{2}^{2}}{\lVert {\Delta} \rVert^{3}} - \frac{1}{\lVert {\Delta} \rVert}\right) + 1 & \text{for}\: \lVert {\Delta} \rVert > \epsilon \wedge \lVert {r_{{t}} \rVert} > \epsilon \\\frac{1}{\lVert {u_{{t}} \rVert}^{3} \mu} \left(1.0 \lVert {u_{{t}} \rVert} \mu u_{{t1}}^{2} - \frac{\mu u_{{t2}}^{2}}{2} \lVert {u_{{t}} \rVert} \theta\left(\lambda^{{\prime\prime}}_{1}\right) - \frac{\mu u_{{t2}}^{2}}{2} \lVert {u_{{t}} \rVert} \theta\left(- 2 \lVert {u_{{t}} \rVert} \mu + \lambda^{{\prime\prime}}_{1}\right) + 1.0 \lVert {u_{{t}} \rVert} \mu u_{{t2}}^{2} - \frac{u_{{t1}}^{2}}{2} \max\left(0, \lambda^{{\prime\prime}}_{1}\right) + \frac{u_{{t1}}^{2}}{2} \max\left(0, - 2 \lVert {u_{{t}} \rVert} \mu + \lambda^{{\prime\prime}}_{1}\right)\right) & \text{for}\: \lVert {r_{{t}} \rVert} \leq \epsilon \wedge \lVert {\Delta} \rVert > \epsilon \wedge \lVert {u_{{t}} \rVert} > \epsilon \end{cases}